src/Ast/FunctionDesugaring.dfy
@@ -1,0 +1,177 @@
+// This module is responsible for
+//   * turning injective function parameters into inverse functions and their corresponding axioms
+//   * creating a tag constant (nullary function) for every tagged function, along with its definition axiom
+//   * declaring a tag axiom for each tagged function
+
+module FunctionDesugaring {
+  import opened Ast
+  import opened Std.Wrappers
+  import opened Basics
+
+  export
+    provides Desugar
+    provides Ast, Wrappers
+
+  method Desugar(b3: Program) returns (r: Result<Program, string>)
+    requires b3.WellFormed()
+    modifies b3.functions
+    ensures r.Success? ==> var r3 := r.value;
+      && b3.types == r3.types
+      && b3.functions <= r3.functions
+      && b3.axioms <= r3.axioms
+      && b3.procedures == r3.procedures
+      && r3.WellFormed()
+  {
+    var functions := b3.functions;
+    var axioms := b3.axioms;
+
+    for i := 0 to |b3.functions|
+      invariant GoodExtension(b3.functions, b3.axioms, functions, axioms)
+    {
+      var func := b3.functions[i];
+      var rr :- AddInverseFunctions(func, b3.functions, b3.axioms, functions, axioms);
+      functions, axioms := rr.0, rr.1;
+      if func.Tag.Some? {
+        rr :- AddFunctionTag(func, b3.functions, b3.axioms, functions, axioms);
+        functions, axioms := rr.0, rr.1;
+      }
+    }
+
+    return Success(Program(b3.types, functions, axioms, b3.procedures));
+  }
+
+  ghost predicate GoodExtension(origFunctions: seq<Function>, origAxioms: seq<Axiom>, functions: seq<Function>, axioms: seq<Axiom>)
+    reads functions
+  {
+    // the new extends the old
+    && origFunctions <= functions
+    && origAxioms <= axioms
+    // properies needed to show the new program is well-formed
+    && (forall func0 <- functions, func1 <- functions :: func0.Name == func1.Name ==> func0 == func1)
+    && (forall func <- functions :: func.WellFormed())
+    && (forall axiom <- axioms :: axiom.WellFormed())
+  }
+
+  method AddInverseFunctions(func: Function, ghost origFunctions: seq<Function>, ghost origAxioms: seq<Axiom>,
+                             functions_in: seq<Function>, axioms_in: seq<Axiom>)
+      returns (r: Result<(seq<Function>, seq<Axiom>), string>)
+    requires func in origFunctions
+    requires GoodExtension(origFunctions, origAxioms, functions_in, axioms_in)
+    modifies func`ExplainedBy
+    ensures r.Success? ==> GoodExtension(origFunctions, origAxioms, r.value.0, r.value.1)
+  {
+    var functions, axioms := functions_in, axioms_in;
+
+    for j := 0 to |func.Parameters|
+      invariant GoodExtension(origFunctions, origAxioms, functions, axioms)
+    {
+      var param := func.Parameters[j];
+      if param.injective {
+        var name := CombineNames(func.Name, param.name);
+        if exists f <- functions :: f.Name == name { // TODO: improve the efficiency of this; there may be a lot of functions in the input, so this matters
+          var msg: string := "function '" + name + "' generated from injective function parameter '" + param.name + "' clashes with an already declared function with that name";
+          return Result<(seq<Function>, seq<Axiom>), string>.Failure(msg);
+        }
+        var parameter := new FParameter("subject", false, func.ResultType);
+        var inverseFunction := new Function(name, [parameter], param.typ, None);
+        functions := functions + [inverseFunction];
+
+        // injectivity axiom:
+        //
+        // axiom explains F
+        //   forall x: X, y: Y pattern F(x, y)
+        //     F.x(F(x, y)) == x
+        var boundVars, pattern, lhs := GenerateAxiomPieces(func, inverseFunction);
+        var rhs := IdExpr(boundVars[j]);
+        var axiom := AssembleAxiom(func, boundVars, pattern, lhs, rhs);
+        axioms := axioms + [axiom];
+      }
+    }
+
+    return Success((functions, axioms));
+  }
+
+  method AddFunctionTag(func: Function, ghost origFunctions: seq<Function>, ghost origAxioms: seq<Axiom>,
+                        functions_in: seq<Function>, axioms_in: seq<Axiom>)
+      returns (r: Result<(seq<Function>, seq<Axiom>), string>)
+    requires func in origFunctions && func.WellFormed() && func.Tag.Some?
+    requires GoodExtension(origFunctions, origAxioms, functions_in, axioms_in)
+    modifies func`ExplainedBy
+    ensures r.Success? ==> GoodExtension(origFunctions, origAxioms, r.value.0, r.value.1)
+  {
+    var functions, axioms := functions_in, axioms_in;
+
+    var name := CombineNames(func.Name, "tag");
+    if exists f: Function <- functions :: f.Name == name { // TODO: improve the efficiency of this; there may be a lot of functions in the input, so this matters
+      var msg: string := "function '" + name + "' generated from the `tag` clause of function '" + func.Name + "' clashes with an already declared function with that name";
+      return Result<(seq<Function>, seq<Axiom>), string>.Failure(msg);
+    }
+
+    // function F.tag(): tag { %tag }
+    var Ftag := new Function(name, [], Types.TagType, None);
+    Ftag.Definition := Some(FunctionDefinition([], CustomLiteral("%tag", Types.TagType)));
+    functions := functions + [Ftag];
+
+    // tag declarations, here shown for function F(x: X, y: Y): S tag G
+    // axiom explains F
+    //   forall x: X, y: Y pattern F(x, y)
+    //     G(F(x, y)) == F.tag()
+    var boundVars, pattern, lhs := GenerateAxiomPieces(func, func.Tag.value);
+    var rhs := FunctionCallExpr(Ftag, []);
+    var axiom := AssembleAxiom(func, boundVars, pattern, lhs, rhs);
+    axioms := axioms + [axiom];
+
+    return Success((functions, axioms));
+  }
+
+  // Given "func" as "function F(x: X, y: Y): S", generate
+  //     * boundVars -- a list of fresh bound variables:  x: X, y: Y
+  //     * pattern -- pattern F(x, y)
+  //     * lhs -- wrapper(F(x, y))
+  method GenerateAxiomPieces(func: Function, wrapper: Function) returns (boundVars: seq<Variable>, pattern: Pattern, lhs: Expr)
+    requires |wrapper.Parameters| == 1
+    ensures |boundVars| == |func.Parameters| && pattern.WellFormed() && lhs.WellFormed()
+  {
+    boundVars := [];
+    for n := 0 to |func.Parameters|
+      invariant |boundVars| == n
+    {
+      var param := func.Parameters[n];
+      var v := new LocalVariable(param.name, false, param.typ);
+      boundVars := boundVars + [v];
+    }
+
+    var Fxy := FunctionCallExpr(func, SeqMap(boundVars, (v: Variable) => IdExpr(v)));
+    pattern := Pattern([Fxy]);
+    lhs := FunctionCallExpr(wrapper, [Fxy]);
+  }
+
+  // Generate:
+  //
+  //     axiom explains func
+  //       forall boundVars
+  //         pattern
+  //         lhs == rhs
+  //
+  // and add this axiom to func.ExplainedBy.
+  method AssembleAxiom(func: Function, boundVars: seq<Variable>, pattern: Pattern, lhs: Expr, rhs: Expr) returns (axiom: Axiom)
+    requires pattern.WellFormed() && lhs.WellFormed() && rhs.WellFormed()
+    modifies func`ExplainedBy
+    ensures axiom.WellFormed()
+  {
+    var body := OperatorExpr(Operator.Eq, [lhs, rhs]);
+    var q;
+    if |boundVars| == 0 {
+      q := body;
+    } else {
+      q := QuantifierExpr(true, boundVars[0]/*TODO: use all the variables*/, [pattern], body);
+    }
+
+    axiom := new Axiom([func], q);
+    func.ExplainedBy := func.ExplainedBy + [axiom];
+  }
+
+  function CombineNames(base: string, member: string): string {
+    base + "." + member
+  }
+}
